src/Where.v
@@ -25,6 +25,281 @@ Import ListNotations.
 Require Import String.
 Open Scope string.
 
+Definition W_expr :=               (EAbs (245,"x")
+             (EIf (EApp
+                   (EApp
+                    (ETApp
+                     (EVar (17,"=="))
+                     (ETyp (TCon (TC TCSeq) [TCon (TC (TCNum 8)) [],TCon (TC TCBit) []])))
+                    (EVar (245,"x")))
+                   (ETApp
+                    (ETApp
+                     (EVar (0,"demote"))
+                     (ETyp (TCon (TC (TCNum 0)) [])))
+                    (ETyp (TCon (TC (TCNum 8)) []))))
+              (EVar (245,"x"))
+              (EApp
+               (EApp
+                (ETApp
+                 (EVar (1,"+"))
+                 (ETyp (TCon (TC TCSeq) [TCon (TC (TCNum 8)) [],TCon (TC TCBit) []])))
+                (ETApp
+                 (ETApp
+                  (EVar (0,"demote"))
+                  (ETyp (TCon (TC (TCNum 1)) [])))
+                 (ETyp (TCon (TC (TCNum 8)) []))))
+               (EApp
+                (EVar (244,"W"))
+                (EApp
+                 (EApp
+                  (ETApp
+                   (EVar (2,"-"))
+                   (ETyp (TCon (TC TCSeq) [TCon (TC (TCNum 8)) [],TCon (TC TCBit) []])))
+                  (EVar (245,"x")))
+                 (ETApp
+                  (ETApp
+                   (EVar (0,"demote"))
+                   (ETyp (TCon (TC (TCNum 1)) [])))
+                  (ETyp (TCon (TC (TCNum 8)) [])))))))).
+
+Definition W_decl :=        [(Recursive
+         [(Decl (244,"W")
+           (DExpr W_expr))])].
+
+Definition rec_id : Expr :=
+     (EAbs (243,"M")
+      (EWhere
+       (EApp
+        (EVar (244,"W"))
+        (EVar (243,"M")))
+       W_decl
+)).
+
+
+(* recursive model of identity *)
+Fixpoint rec_model (fuel : nat) (e : ext_val) : ext_val :=
+  match fuel with
+  | O => e
+  | S fuel' =>
+    match e with
+    | eseq l =>
+      match to_bitv l with
+      | Some bv => rec_model fuel' (eseq (@from_bitv (Datatypes.length l) (add bv mone)))
+      | None => eseq nil
+      end
+    | _ => eseq nil
+    end
+  end.
+
+Definition extnum (val width : Z) : list ext_val :=
+  ExtToBitvector.from_bitv (@repr (Z.to_nat width) val).
+
+Lemma tobit_frombit_id :
+  forall {w} (bv : BitV w),
+    to_bitv (from_bitv bv) = Some bv.
+Proof.
+Admitted.
+
+Lemma from_bitv_length :
+  forall w (bv : BitV w),
+    Datatypes.length (@from_bitv w bv) = w.
+Proof.
+Admitted.
+
+Lemma eval_W_id :
+  forall n GE TE SE,
+    GE (244,"W") = Some W_expr ->
+    SE (244,"W") = None ->
+    GE (17,"==") = Some (mb 1 2 Eq) ->
+    SE (17,"==") = None ->
+    GE (1,"+") = Some (mb 1 2 Plus) ->
+    SE (1,"+") = None ->
+    GE (2,"-") = Some (mb 1 2 Minus) ->
+    SE (2,"-") = None ->
+    GE (0,"demote") = Some (mb 2 0 Demote) ->
+    SE (0,"demote") = None ->
+    forall l bv,
+      has_type (eseq l) (tseq 8 tbit) ->
+      @to_bitv (Datatypes.length l) l = Some bv ->
+      n = Z.to_nat (unsigned bv) ->
+      forall argexp res,
+        eager_eval_expr GE TE SE argexp (to_sval (eseq l)) ->
+        res = to_sval (rec_model n (eseq l)) ->
+        eager_eval_expr GE TE SE (EApp (EVar (244,"W")) argexp) res.
+Proof.
+  induction n; intros.
+
+  * e. ag. e. e. 
+    use eq_eval.
+    instantiate (1 := eseq l).
+    lv.
+    instantiate (1 := eseq (repeat (ebit false) 8)).
+    simpl.
+    use demote_eval.
+    instantiate (1 := true).
+    admit. (* We have enough information *)
+
+    simpl. subst res. unfold rec_model.
+    lv.
+  *
+    assert (Hlen : Datatypes.length l = 8%nat). {
+      inversion H9; eauto.
+    } 
+    
+    e. ag. e. e.
+    use eq_eval.
+    
+    instantiate (1 := eseq l).
+    lv.
+    instantiate (1 := eseq (repeat (ebit false) 8)).
+    simpl.
+    use demote_eval.
+    instantiate (1 := false).
+    admit. (* We have enough information *)
+    simpl.
+    eapply plus_eval.
+    intuition; eassumption.
+    unfold extend; simpl; intuition; eassumption.
+    et.
+    use demote_eval.
+    simpl.
+
+    instantiate (1 := (extnum 1 8)).
+    reflexivity.
+
+    eapply IHn.
+    intuition; eassumption.
+    intuition; eassumption.
+    intuition; eassumption.
+    intuition; eassumption.
+    intuition; eassumption.
+    intuition; eassumption.
+    intuition; eassumption.
+    intuition; eassumption.
+    intuition; eassumption.
+    intuition; eassumption.
+    Focus 4.
+    eapply minus_eval.
+    intuition; eassumption.
+    intuition; eassumption.
+    et. lv.
+    use demote_eval.
+    instantiate (1 := extnum 1 8).
+    reflexivity.
+    eassumption.
+    unfold extnum.
+    instantiate (1 := repr 1).
+    repeat rewrite Hlen.
+    rewrite tobit_frombit_id.
+    reflexivity.
+    reflexivity.
+    admit. (* it's true, just type *)
+    simpl.
+
+    (* we want (bv - 1) *)
+    (* but dependent types are awful *)
+    
+    admit.
+    admit.
+
+    f_equal.
+    unfold rec_model.
+
+    (* It all works, modulo bit widths being terrible *)
+    (* dependent types are kinda the worst *)
+
+    (* TODO: rewrite semantics of add/sub/mul/etc to not use BitV *)
+    (* BitV makes reasoning about these programs too complicated *)
+    (* It would be much easier with simple types and options *)
+Admitted.
+
+
+Lemma eval_rec_id :
+  forall n GE TE SE,
+    GE (244,"W") = Some W_expr ->
+    SE (244,"W") = None ->
+    GE (17,"==") = Some (mb 1 2 Eq) ->
+    SE (17,"==") = None ->
+    GE (1,"+") = Some (mb 1 2 Plus) ->
+    SE (1,"+") = None ->
+    GE (2,"-") = Some (mb 1 2 Minus) ->
+    SE (2,"-") = None ->
+    GE (0,"demote") = Some (mb 2 0 Demote) ->
+    SE (0,"demote") = None ->
+    forall l bv,
+      has_type (eseq l) (tseq 8 tbit) ->
+      @to_bitv (Datatypes.length l) l = Some bv ->
+      n = Z.to_nat (unsigned bv) ->
+      forall argexp res,
+        eager_eval_expr GE TE SE argexp (to_sval (eseq l)) ->
+        res = to_sval (rec_model n (eseq l)) ->
+        eager_eval_expr GE TE SE (EApp rec_id argexp) res.
+Proof.
+  induction n; intros.
+
+  * e. e. e. e. g. e. lv.
+    e.
+    use eq_eval.
+    instantiate (1 := eseq l).
+    lv.
+    instantiate (1 := eseq (repeat (ebit false) 8)).
+    simpl.
+    use demote_eval.
+    instantiate (1 := true).
+    admit. (* We have enough information *)
+
+    simpl. subst res. unfold rec_model.
+    lv.
+  *
+    assert (Hlen : Datatypes.length l = 8%nat). {
+      inversion H9; eauto.
+    } 
+    
+    e. e. e. e. g. e. lv.
+    e.
+    use eq_eval.
+    
+    instantiate (1 := eseq l).
+    lv.
+    instantiate (1 := eseq (repeat (ebit false) 8)).
+    simpl.
+    use demote_eval.
+    instantiate (1 := false).
+    admit. (* We have enough information *)
+    simpl.
+    eapply plus_eval.
+    intuition; eassumption.
+    unfold extend; simpl; intuition; eassumption.
+    et.
+    use demote_eval.
+    simpl.
+
+    instantiate (1 := (extnum 1 8)).
+    reflexivity.
+
+    e. g. e.
+    eapply minus_eval.
+    intuition; eassumption.
+    unfold extend; simpl; intuition; eassumption.
+    et.
+    instantiate (1 := l). lv.
+    instantiate (1 := extnum 1 8).
+    use demote_eval. rewrite H10. reflexivity.
+    instantiate (1 := @repr (Datatypes.length l) 1).
+    rewrite Hlen. reflexivity.
+    reflexivity.
+    
+    
+
+    
+  
+Qed.
+    
+
+
+
+
+    
 
 Definition where_test : Expr :=
   (EAbs (243,"M")
